#### \*1. Negate these statements and then reexpress the results as equivalent positive statements. (See Example 2.2.1.)

- (a) Everyone who is majoring in math has a friend who needs help with his homework.

  Let $M(x)$ be "$x$ is majoring in math", $H(x)$ be "$x$ needs help with his homework", and $F(x,y)$ be "$x$ is a friend of $y$".

  Then we have the statement in (a) expressed as $\forall x \Big[M(x) \longrightarrow \exist y\big(F(x, y) \land H(y)\big)\Big]$

  $\neg\forall x \Big[M(x) \longrightarrow \exist y\big(F(x, y) \land H(y)\big)\Big]$

  $\exist x \neg\Big[\neg M(x) \lor \exist y\big(F(x, y) \land H(y)\big)\Big]$

  $\exist x \Big[ M(x) \land \neg\exist y\big(F(x, y) \land H(y)\big)\Big]$

  $\exist x \Big[ M(x) \land \forall y\big(\neg F(x, y) \lor \neg H(y)\big)\Big]$

- (b) Everyone has a roommate who dislikes everyone.

  Let $R(x,y)$ be "$x$ is a roommate of $y$", $L(x, y)$ be "$x$ likes $y$"

  $\forall x \exist y(R(x,y) \longrightarrow \forall z \neg L(y, z))$

  Then

  $\neg\Bigg[\Big(\forall x \exist y(R(x,y) \longrightarrow \forall z \neg L(y, z)\Big)\Bigg]$

  $\exist x \neg\exist y(R(x,y) \longrightarrow \forall z \neg L(y, z))$

  $\exist x \forall y\neg(\neg R(x,y) \lor \forall z \neg L(y, z))$

  $\exist x \forall y(R(x,y) \land \neg\forall z \neg L(y, z))$

  $\exist x \forall y(R(x,y) \land \exist z L(y, z))$

* (c) $A \cup B \subseteq C \setminus D$.-
* $=\neg\forall x\Bigg[\Big(x\- in A \lor x\in B\Big)\longrightarrow\Big(x\in C \land x\notin D\Big)\Bigg]$-

  $\exist x\neg\Bigg[\neg\Big(x\in A \lor x\in B\Big)\lor\Big(x\in C \land x\notin D\Big)\Bigg]$

  $\exist x\Bigg[\Big(x\in A \lor x\in B\Big)\land\neg\Big(x\in C \land x\notin D\Big)\Bigg]$

  $\exist x\Bigg[\Big(x\in A \lor x\in B\Big)\land\Big(x\notin C \lor x\in D\Big)\Bigg]$

* (d) $\exist x \forall y [y \gt x \longrightarrow \exist z(z^2 + 5z = y)]$.

  $=\neg\exist x \forall y [y \gt x \longrightarrow \exist z(z^2 + 5z = y)]$

  $\forall x \neg\forall y [y \gt x \longrightarrow \exist z(z^2 + 5z = y)]$

  $\forall x \exist y \neg[y \lt x \lor \exist z(z^2 + 5z = y)]$

  $\forall x \exist y [y \gt x \land \neg\exist z(z^2 + 5z = y)]$

  $\forall x \exist y [y \gt x \land \forall z\neg(z^2 + 5z = y)]$

  $\forall x \exist y [y \gt x \land \forall z(z^2 + 5z \neq y)]$

#### 2. Negate these statements and then reexpress the results as equivalent positive statements. (See Example 2.2.1.)

- (a) There is someone in the freshman class who doesnâ€™t have a roommate.

  Let $F(x)$ be "$x$ is in the freshman class", $R(x,y)$ be "$x$ and $y$ are roommates"

  Then we have $\exist x\Big[F(x)\land \forall y\neg R(x,y)\Big]$

  $\neg\exist x\Big[F(x)\land \forall y\neg R(x,y)\Big]$

  $\forall x\Big[\neg F(x)\lor \exist y R(x,y)\Big]$

  $\forall x\Big[F(x)\implies \exist y R(x,y)\Big]$

  For everyone who is in the freshman class, there is at least one person who has a roommate.

- (b) Everyone likes someone, but no one likes everyone.

  Let $L(x,y)$ be "$x$ likes $y$", then

  $\forall x \exist y\Big(L(x,y) \Big)\land \neg\exist x\forall y\Big(L(x,y)\Big)$

  $\neg\Bigg[\forall x \exist y\Big(L(x,y) \Big)\land \neg\exist x\forall y\Big(L(x,y)\Big)\Bigg]$

  $\neg\forall x \exist y\Big(L(x,y) \Big)\lor\neg\neg\exist x\forall y\Big(L(x,y)\Big)$

  $\exist x \neg\exist y\Big(L(x,y) \Big)\lor\exist x\forall y\Big(L(x,y)\Big)$

  $\exist x \exist y\neg L(x,y) \lor\exist x\forall y L(x,y)$

  Either there is at least one person $x$, who dislikes a different person $y$, or that person $x$ likes everyone.

- (c) $\forall a \in A\exist b \in B(a \in C \iff b\in C)$.

  $\forall a\Bigg( a \in A\implies\exist b \Big(b\in B \implies (a \in C \iff b\in C)\Big)\Bigg)$

  $\forall a\Bigg( a \in A\implies\exist b \Big(b\in B \implies (a \in C \implies b \in C) \land (B\in C \implies a \in C)\Big)\Bigg)$

  $\forall a\Bigg( a \notin A\lor\exist b \Big(b\notin B \lor (a \notin C \lor b \in C) \land (b\notin C \lor a \in C)\Big)\Bigg)$

  Then

  $\neg \forall a\Bigg( a \notin A\lor\exist b \Big(b\notin B \lor ((a \notin C \lor b \in C) \land (b\notin C \lor a \in C)\Big)\Bigg)$

  $\exist a\neg\Bigg( a \notin A\lor\exist b \Big(b\notin B \lor ((a \notin C \lor b \in C) \land (b\notin C \lor a \in C))\Big)\Bigg)$ (quantifier negation)

  $\exist a\Bigg( a \in A\land \neg\exist b \Big(b\notin B \lor ((a \notin C \lor b \in C) \land (b\notin C \lor a \in C))\Big)\Bigg)$ (DeMorgan's law)

  $\exist a\Bigg( a \in A\land \forall b \neg\Big(b\notin B \lor ((a \notin C \lor b \in C) \land (b\notin C \lor a \in C))\Big)\Bigg)$ (quantifier negation)

  $\exist a\Bigg( a \in A\land \forall b \Big(b\in B \land ((a \in C \land b \notin C) \lor (b\in C \land a \notin C))\Big)\Bigg)$ (DeMorgan's law)$^3$

- (d) $\forall y \gt 0 \exist x (ax^2 + bx + c =y)$.

  $\forall y (y\gt 0 \implies \exist x (ax^2 + bx + c =y))$ (expand)

  Then

  $\neg\forall y (y\gt 0 \implies \exist x (ax^2 + bx + c =y))$

  $\exist y \neg(\neg(y\gt 0) \lor \neg\exist x (ax^2 + bx + c =y))$

  $\exist y \neg(y\lt 0 \lor \forall x \neg(ax^2 + bx + c =y))$

  $\exist y \neg(y\lt 0 \lor \forall x (ax^2 + bx + c \neq y))$

  $\exist y (\neg(y\lt 0) \land \neg\forall x (ax^2 + bx + c \neq y))$

  $\exist y (y\gt 0 \land \exist x \neg (ax^2 + bx + c \neq y))$

  $\exist y (y\gt 0 \land \exist x (ax^2 + bx + c = y))$

#### 3. Are these statements true or false? The universe of discourse is $\N$.

- (a) $\exist x(x \lt 7 \implies \exist a \exist b \exist c(a^2+b^2+c^2=x))$.

  $x\in\{0,1,2,3,4,5,6\}$, since our statement does not state that $a$, $b$ or $c$ have to be different, with $x=6$ and $a=b=1,c=2$, the equation $a^2+b^2+c^2=x$ is true ($1+1+4=6$).

- (b) $\exist!x((x-4)^2=9)$.
  - True, since $9$ is a perfect square, there is only one value for which $(x-4)^2=9$, which would be $x=7$
- (c) $\exist!x((x-4)^2=25)$.
  - True, for the same reason as (b): only one value for $x\in\N$ satisfies $(x-4)^2=25$
- (d) $\exist x \exist y ((x-4)^2=25\land(y-5)^2=2)$.
  - False, as there is no $y\in\N$ that satisfies $(y-5)^2=2$

#### \*4. Show that the second quantifier negation law, which says that $\neg \forall x P(x)$ is equivalent to $\exist x \neg P(x)$, can be derived from the first, which says that $\neg \exist x P(x)$ is equivalent to $\forall x \neg P(x)$. (Hint: Use the double negation law.)

$\neg \exist x P(x) \equiv\forall x \neg P(x)$

$\neg\Big(\neg \exist x P(x) \Big) \equiv\neg\Big(\forall x \neg P(x)\Big)$

$\neg\neg \exist x P(x) \equiv\neg\forall x \neg P(x)$

$\neg\neg \exist x P(x) \equiv \exist x \neg\neg P(x)$

$\exist x P(x) \equiv \exist x \neg\neg P(x)$

#### \*6. Show that the existential quantifier distributes over disjunction. In other words, show that $\exist x\Big(P(x)\lor Q(x)\Big)$ is equivalent to $\exist x P(x)\lor \exist x Q(x)$. (Hint: Use the fact, discussed in this section, that the universal quantifier distributes over conjunction.)

Show that

$\exist x\Big(P(x)\lor Q(x)\Big) \equiv\exist x P(x)\lor \exist x Q(x)$

Negating both sides of the equivalence

$\neg\exist x\Big(P(x)\lor Q(x)\Big) \equiv\neg\Big[\exist x P(x)\lor \exist x Q(x)\Big]$

$\forall x\neg\Big(P(x)\lor Q(x)\Big) \equiv\neg\Big[\exist x P(x)\lor \exist x Q(x)\Big]$

$\forall x\Big(\neg P(x)\land \neg Q(x)\Big) \equiv\neg\Big[\exist x P(x)\lor \exist x Q(x)\Big]$

$\forall x\neg P(x)\land \forall x\neg Q(x) \equiv\neg\Big[\exist x P(x)\lor \exist x Q(x)\Big]$

Using the quantifier negation laws once more

$\neg\exist x P(x)\land \neg\exist x Q(x) \equiv\neg\Big[\exist x P(x)\lor \exist x Q(x)\Big]$

Through DeMorgan's law

$\neg\Big[\exist x P(x)\lor \exist x Q(x) \Big]\equiv\neg\Big[\exist x P(x)\lor \exist x Q(x)\Big]$

$\neg\neg\Big[\exist x P(x)\lor \exist x Q(x) \Big]\equiv\neg\neg\Big[\exist x P(x)\lor \exist x Q(x)\Big]$

$\exist x P(x)\lor \exist x Q(x) \equiv \exist x P(x)\lor \exist x Q(x)$

#### 7. Show that $\exist x \Big(P(x)\implies Q(x)\Big)$ is equivalent to $\forall x p(x)\implies\exist x Q(x)$.

$\exist x \Big(P(x)\implies Q(x)\Big) \equiv \forall x P(x)\implies\exist x Q(x)$

$\exist x \Big(\neg P(x)\lor Q(x)\Big) \equiv \forall x P(x)\implies\exist x Q(x)$

Substituting $\neg P(x)\lor Q(x)$ by its DeMorgan equivalent $\neg(P(x)\land\neg Q(x))$

$\exist x \neg\Big( P(x)\land \neg Q(x)\Big) \equiv \forall x P(x)\implies\exist x Q(x)$

$\neg\forall x \Big( P(x)\land \neg Q(x)\Big) \equiv \forall x P(x)\implies\exist x Q(x)$

Since the universal quantifier distributes over conjunction

$\neg\Big[\forall x P(x)\land \forall x \neg Q(x)\Big] \equiv \forall x P(x)\implies\exist x Q(x)$

$\neg\Big[\forall x P(x)\land \neg\exist x  Q(x)\Big] \equiv \forall x P(x)\implies\exist x Q(x)$

DeMorgan's law:

$\neg\forall x P(x)\lor \neg\neg\exist x  Q(x) \equiv \forall x P(x)\implies\exist x Q(x)$

$\neg\forall x P(x)\lor \exist x  Q(x) \equiv \forall x P(x)\implies\exist x Q(x)$

Conditional law ( $P\implies Q \equiv \neg P \lor Q$ )

$\forall x P(x)\implies \exist x  Q(x) \equiv \forall x P(x)\implies\exist x Q(x)$

#### \*8. Show that $(\forall x \in A P(x))\land (\forall x  \in B P(x))$ is equivalent to $\forall x \in (A\cup B)P(x)$. (Hint: Start by writing out the meanings of the bounded quantifiers in terms of unbounded quantifiers.)

$(\forall x \in A P(x))\land (\forall x  \in B P(x)) \equiv \forall x \in (A\cup B)P(x)$.

$(\forall x(x \in A \implies P(x)))\land (\forall x (x \in B \implies P(x))) \equiv \forall x \in (A\cup B)P(x)$. (expand)

$\forall x(x \notin A \lor P(x))\land \forall x (x \notin B \lor P(x)) \equiv \forall x \in (A\cup B)P(x)$. (conditional law)

$\forall x\Big[(x \notin A \lor P(x))\land (x \notin B \lor P(x))\Big] \equiv \forall x \in (A\cup B)P(x)$. (distribute over conjunction)

$\forall x\Big[\Big(x \notin A \land x \notin B\Big)\lor P(x)\Big] \equiv \forall x \in (A\cup B)P(x)$. (distribute law)

$\forall x\Big[\neg\Big(x \in A \lor x \in B\Big)\lor P(x)\Big] \equiv \forall x \in (A\cup B)P(x)$. (DeMorgan's law)

$\forall x\Big[\neg\Big(x \in (A \cup B)\Big)\lor P(x)\Big] \equiv \forall x \in (A\cup B)P(x)$. (Definition of $\cup$)

$\forall x\Big[x \in (A \cup B)\implies P(x)\Big] \equiv \forall x \in (A\cup B)P(x)$. (Definition of $\implies$)

$\forall x\in (A \cup B) P(x) \equiv \forall x \in (A\cup B)P(x)$. (abbreviate)

#### 9. Is $\forall x(P(x) \lor Q(x))$ equivalent to $\forall x P(x) \lor \forall xQ(x)$? Explain. (Hint: Try assigning meanings to $P(x)$ and $Q(x)$.)

Let $P(x)$ be "x flag has the color red", and $Q(x)$ be "$x$ flag has the color blue", then our statements become

$\forall x(P(x) \lor Q(x))=$ all flags have either the color red or the color blue

$\forall x P(x) \lor \forall xQ(x)=$ Either all flags have the color red, or all flags have the color blue
