# Chapter 2.2 Notes

## Quantifier negation laws (P. 68)

$\neg \exists x P(x)\qquad \equiv \qquad \forall x \neg P(x)$

$\neg \forall P(x) \qquad \equiv \qquad \exists x \neg P(x)$


## Quantifier distribution

### Universal quantifier distributes over conjunction.

> ... Thus, it appears that $\forall x (E(x)\land T(x)) \equiv \forall x E(x) \land \forall x T(x)$. In other words, we conclude that *the universal quantifier distributes over conjunction*.
â€” Page 74

### Existencial quantifier distribution over disjunction

This is proved in exercise 2.2.6:

$\exists x\Big(P(x)\lor Q(x)\Big) \equiv\exists x P(x)\lor \exists x Q(x)$

Negating both sides of the equivalence

$\neg\exists x\Big(P(x)\lor Q(x)\Big) \equiv\neg\Big(\exists x P(x)\lor \exists x Q(x)\Big)$

$\forall x\neg\Big(P(x)\lor Q(x)\Big) \equiv\neg\Big(\exists x P(x)\lor \exists x Q(x)\Big)$

$\forall x\Big(\neg P(x)\land \neg Q(x)\Big) \equiv\neg\Big(\exists x P(x)\lor \exists x Q(x)\Big)$

$\forall x\neg P(x)\land \forall x\neg Q(x) \equiv\neg\Big(\exists x P(x)\lor \exists x Q(x)\Big)$

Using the quantifier negation laws once more

$\neg\exists x P(x)\land \neg\exists x Q(x) \equiv\neg\Big(\exists x P(x)\lor \exists x Q(x)\Big)$

Through DeMorgan's law

$\neg\Big(\exists x P(x)\lor \exists x Q(x) \Big)\equiv\neg\Big(\exists x P(x)\lor \exists x Q(x)\Big)$

$\neg\neg\Big(\exists x P(x)\lor \exists x Q(x) \Big)\equiv\neg\neg\Big(\exists x P(x)\lor \exists x Q(x)\Big)$

$\exists x P(x)\lor \exists x Q(x) \equiv \exists x P(x)\lor \exists x Q(x)$



