# Chapter 2.2

#### \*1. Negate these statements and then reexpress the results as equivalent positive statements. (See Example 2.2.1.)

- (a) Everyone who is majoring in math has a friend who needs help with his homework.

  Let $M(x)$ be "$x$ is majoring in math", $H(x)$ be "$x$ needs help with his homework", and $F(x,y)$ be "$x$ is a friend of $y$".

  Then we have the statement in (a) expressed as 
  
  $$\forall x \Big(M(x) \longrightarrow \exists y\big(F(x, y) \land H(y)\big)\Big)$$

Negating this statement:

  $$\neg\forall x \Big(M(x) \longrightarrow \exists y\big(F(x, y) \land H(y)\big)\Big)$$

  $$\exists x \neg\Big(\neg M(x) \lor \exists y\big(F(x, y) \land H(y)\big)\Big)$$

  $$\exists x \Big( M(x) \land \neg\exists y\big(F(x, y) \land H(y)\big)\Big)$$

  $$\exists x \Big( M(x) \land \forall y\neg\big(F(x, y) \land H(y)\big)\Big)$$

  $$\exists x \Big( M(x) \land \forall y\big(\neg F(x, y) \lor \neg H(y)\big)\Big)$$

  There is someone majoring in math, and everyone who is not their friend, does not need help with their homework.

- (b) Everyone has a roommate who dislikes everyone.

  Let $R(x,y)$ be "$x$ is a roommate of $y$", $L(x, y)$ be "$x$ likes $y$"

  $\forall x \exists y(R(x,y) \longrightarrow \forall z \neg L(y, z))$

  Then

  $\neg\Bigg[\Big(\forall x \exists y(R(x,y) \longrightarrow \forall z \neg L(y, z)\Big)\Bigg]$

  $\exists x \neg\exists y(R(x,y) \longrightarrow \forall z \neg L(y, z))$

  $\exists x \forall y\neg(\neg R(x,y) \lor \forall z \neg L(y, z))$

  $\exists x \forall y(R(x,y) \land \neg\forall z \neg L(y, z))$

  $\exists x \forall y(R(x,y) \land \exists z L(y, z))$

* (c) $A \cup B \subseteq C \setminus D$

  $\forall x \Big( x\in (A \cup B) \longrightarrow x \in (C \setminus D) \Big)$

  $\forall x \Big( \big(x\in A \lor x \in B\big) \longrightarrow \big(x \in C \land x \notin D \big) \Big)$

  $\forall x \Big( \neg\big(x\in A \lor x \in B\big) \lor \big(x \in C \land x \notin D \big) \Big)$

  Negating:

  $\neg\forall x \Big( \neg\big(x\in A \lor x \in B\big) \lor \big(x \in C \land x \notin D \big) \Big)$

  $\exists x \neg\Big( \neg\big(x\in A \lor x \in B\big) \lor \big(x \in C \land x \notin D \big) \Big)$

  $\exists x \Big( \big(x\in A \lor x \in B\big) \land \neg\big(x \in C \land x \notin D \big) \Big)$

  $\exists x \Big( \big(x\in A \lor x \in B\big) \land \big(x \in D \lor x \notin C \big) \Big)$

  $\exists x \Big( \neg\big(x\notin A \land x \notin B\big) \land \big(x \in D \lor x \notin C \big) \Big)$

  $\exists x \Big( x\notin A \cap  B \longrightarrow x \in D \setminus  C \Big)$


* (d) $\exists x \forall y [y > x \longrightarrow \exists z(z^2 + 5z = y)]$.

  $=\neg\exists x \forall y [y > x \longrightarrow \exists z(z^2 + 5z = y)]$

  $\forall x \neg\forall y [y > x \longrightarrow \exists z(z^2 + 5z = y)]$

  $\forall x \exists y \neg[y < x \lor \exists z(z^2 + 5z = y)]$

  $\forall x \exists y [y > x \land \neg\exists z(z^2 + 5z = y)]$

  $\forall x \exists y [y > x \land \forall z\neg(z^2 + 5z = y)]$

  $\forall x \exists y [y > x \land \forall z(z^2 + 5z \neq y)]$

#### 2. Negate these statements and then reexpress the results as equivalent positive statements. (See Example 2.2.1.)

- (a) There is someone in the freshman class who doesnâ€™t have a roommate.

  Let $F(x)$ be "$x$ is in the freshman class", $R(x,y)$ be "$x$ and $y$ are roommates"

  Then we have $\exists x\Big( F(x) \land \forall y \neg R(x,y) \Big)$

  $\neg\exists x\Big(F(x)\land \forall y\neg R(x,y)\Big)$

  $\forall x\Big(\neg F(x)\lor \exists y R(x,y)\Big)$

  $\forall x\Big(F(x)\implies \exists y R(x,y)\Big)$

  For everyone who is in the freshman class, there is at least one person who has a roommate.

- (b) Everyone likes someone, but no one likes everyone.

  Let $L(x,y)$ be "$x$ likes $y$", then

  $\forall x \exists y\Big(L(x,y) \Big)\land \neg\exists x\forall y\Big(L(x,y)\Big)$

  $\neg\Bigg[\forall x \exists y\Big(L(x,y) \Big)\land \neg\exists x\forall y\Big(L(x,y)\Big)\Bigg]$

  $\neg\forall x \exists y\Big(L(x,y) \Big)\lor\neg\neg\exists x\forall y\Big(L(x,y)\Big)$

  $\exists x \neg\exists y\Big(L(x,y) \Big)\lor\exists x\forall y\Big(L(x,y)\Big)$

  $\exists x \exists y\neg L(x,y) \lor\exists x\forall y L(x,y)$

  Either there is at least one person $x$, who dislikes a different person $y$, or that person $x$ likes everyone.

- (c) $\forall a \in A\exists b \in B(a \in C \iff b\in C)$.

  $\forall a\Bigg( a \in A\implies\exists b \Big(b\in B \implies (a \in C \iff b\in C)\Big)\Bigg)$

  $\forall a\Bigg( a \in A\implies\exists b \Big(b\in B \implies (a \in C \implies b \in C) \land (B\in C \implies a \in C)\Big)\Bigg)$

  $\forall a\Bigg( a \notin A\lor\exists b \Big(b\notin B \lor (a \notin C \lor b \in C) \land (b\notin C \lor a \in C)\Big)\Bigg)$

  Then

  $\neg \forall a\Bigg( a \notin A\lor\exists b \Big(b\notin B \lor ((a \notin C \lor b \in C) \land (b\notin C \lor a \in C)\Big)\Bigg)$

  $\exists a\neg\Bigg( a \notin A\lor\exists b \Big(b\notin B \lor ((a \notin C \lor b \in C) \land (b\notin C \lor a \in C))\Big)\Bigg)$ (quantifier negation)

  $\exists a\Bigg( a \in A\land \neg\exists b \Big(b\notin B \lor ((a \notin C \lor b \in C) \land (b\notin C \lor a \in C))\Big)\Bigg)$ (DeMorgan's law)

  $\exists a\Bigg( a \in A\land \forall b \neg\Big(b\notin B \lor ((a \notin C \lor b \in C) \land (b\notin C \lor a \in C))\Big)\Bigg)$ (quantifier negation)

  $\exists a\Bigg( a \in A\land \forall b \Big(b\in B \land ((a \in C \land b \notin C) \lor (b\in C \land a \notin C))\Big)\Bigg)$ (DeMorgan's law)$^3$

- (d) $\forall y > 0 \exists x (ax^2 + bx + c =y)$.

  $\forall y (y> 0 \implies \exists x (ax^2 + bx + c =y))$ (expand)

  Then

  $\neg\forall y (y> 0 \implies \exists x (ax^2 + bx + c =y))$

  $\exists y \neg(\neg(y> 0) \lor \neg\exists x (ax^2 + bx + c =y))$

  $\exists y \neg(y< 0 \lor \forall x \neg(ax^2 + bx + c =y))$

  $\exists y \neg(y< 0 \lor \forall x (ax^2 + bx + c \neq y))$

  $\exists y (\neg(y< 0) \land \neg\forall x (ax^2 + bx + c \neq y))$

  $\exists y (y> 0 \land \exists x \neg (ax^2 + bx + c \neq y))$

  $\exists y (y> 0 \land \exists x (ax^2 + bx + c = y))$

#### 3. Are these statements true or false? The universe of discourse is $\mathbb{N}$.

- (a) $\exists x(x < 7 \implies \exists a \exists b \exists c(a^2+b^2+c^2=x))$.

  $x\in\{-\infty,\ldots, 0,1,2,3,4,5,6\}$, since our statement does not state that $a$, $b$ or $c$ have to be different, with $x=6$ and $a=b=1,c=2$, the equation $a^2+b^2+c^2=x$ is true ($1+1+4=6$).

- (b) $\exists!x((x-4)^2=9)$.
  - True, since $9$ is a perfect square, there is only one value in $\mathbb{N}$ for which $(x-4)^2=9$, which would be $x=7$
- (c) $\exists!x((x-4)^2=25)$.
  - True, for the same reason as (b): only one value for $x\in\mathbb{N}$ satisfies $(x-4)^2=25$
- (d) $\exists x \exists y ((x-4)^2=25\land(y-5)^2=2)$.
  - False, as there is no $y\in\mathbb{N}$ that satisfies $(y-5)^2=2$

#### \*4. Show that the second quantifier negation law, which says that $\neg \forall x P(x)$ is equivalent to $\exists x \neg P(x)$, can be derived from the first, which says that $\neg \exists x P(x)$ is equivalent to $\forall x \neg P(x)$. (Hint: Use the double negation law.)

$\neg \exists x P(x) \equiv\forall x \neg P(x)$

$\neg\Big(\neg \exists x P(x) \Big) \equiv\neg\Big(\forall x \neg P(x)\Big)$

$\neg\neg \exists x P(x) \equiv\neg\forall x \neg P(x)$

$\neg\neg \exists x P(x) \equiv \exists x \neg\neg P(x)$

$\exists x P(x) \equiv \exists x \neg\neg P(x)$

$\exists x P(x) \equiv \exists x P(x)$

#### \*6. Show that the existential quantifier distributes over disjunction. In other words, show that $\exists x\Big(P(x)\lor Q(x)\Big)$ is equivalent to $\exists x P(x)\lor \exists x Q(x)$. (Hint: Use the fact, discussed in this section, that the universal quantifier distributes over conjunction.)

Show that

$\exists x\Big(P(x)\lor Q(x)\Big) \equiv\exists x P(x)\lor \exists x Q(x)$

Negating both sides of the equivalence

$\neg\exists x\Big(P(x)\lor Q(x)\Big) \equiv\neg\Big(\exists x P(x)\lor \exists x Q(x)\Big)$

$\forall x\neg\Big(P(x)\lor Q(x)\Big) \equiv\neg\Big(\exists x P(x)\lor \exists x Q(x)\Big)$

$\forall x\Big(\neg P(x)\land \neg Q(x)\Big) \equiv\neg\Big(\exists x P(x)\lor \exists x Q(x)\Big)$

$\forall x\neg P(x)\land \forall x\neg Q(x) \equiv\neg\Big(\exists x P(x)\lor \exists x Q(x)\Big)$

Using the quantifier negation laws once more

$\neg\exists x P(x)\land \neg\exists x Q(x) \equiv\neg\Big(\exists x P(x)\lor \exists x Q(x)\Big)$

Through DeMorgan's law

$\neg\Big(\exists x P(x)\lor \exists x Q(x) \Big)\equiv\neg\Big(\exists x P(x)\lor \exists x Q(x)\Big)$

$\neg\neg\Big(\exists x P(x)\lor \exists x Q(x) \Big)\equiv\neg\neg\Big(\exists x P(x)\lor \exists x Q(x)\Big)$

$\exists x P(x)\lor \exists x Q(x) \equiv \exists x P(x)\lor \exists x Q(x)$

#### 7. Show that $\exists x \Big(P(x)\implies Q(x)\Big)$ is equivalent to $\forall x P(x)\implies\exists x Q(x)$.

$\exists x \Big(P(x)\implies Q(x)\Big) \equiv \forall x P(x)\implies\exists x Q(x)$

$\exists x \Big(\neg P(x)\lor Q(x)\Big) \equiv \forall x P(x)\implies\exists x Q(x)$

Substituting $\neg P(x)\lor Q(x)$ by its DeMorgan equivalent $\neg(P(x)\land\neg Q(x))$

$\exists x \neg\Big( P(x)\land \neg Q(x)\Big) \equiv \forall x P(x)\implies\exists x Q(x)$

$\neg\forall x \Big( P(x)\land \neg Q(x)\Big) \equiv \forall x P(x)\implies\exists x Q(x)$

Since the universal quantifier distributes over conjunction

$\neg\Big(\forall x P(x)\land \forall x \neg Q(x)\Big) \equiv \forall x P(x)\implies\exists x Q(x)$

$\neg\Big(\forall x P(x)\land \neg\exists x  Q(x)\Big) \equiv \forall x P(x)\implies\exists x Q(x)$

DeMorgan's law:

$\neg\forall x P(x)\lor \neg\neg\exists x  Q(x) \equiv \forall x P(x)\implies\exists x Q(x)$

$\neg\forall x P(x)\lor \exists x  Q(x) \equiv \forall x P(x)\implies\exists x Q(x)$

Conditional law ( $P\implies Q \equiv \neg P \lor Q$ )

$\forall x P(x)\implies \exists x  Q(x) \equiv \forall x P(x)\implies\exists x Q(x)$

#### \*8. Show that $(\forall x \in A P(x))\land (\forall x  \in B P(x))$ is equivalent to $\forall x \in (A\cup B)P(x)$. (Hint: Start by writing out the meanings of the bounded quantifiers in terms of unbounded quantifiers.)

$(\forall x \in A P(x))\land (\forall x  \in B P(x)) \equiv \forall x \in (A\cup B)P(x)$.

$(\forall x(x \in A \implies P(x)))\land (\forall x (x \in B \implies P(x))) \equiv \forall x \in (A\cup B)P(x)$. (expand)

$\forall x(x \notin A \lor P(x))\land \forall x (x \notin B \lor P(x)) \equiv \forall x \in (A\cup B)P(x)$. (conditional law)

$\forall x\Big((x \notin A \lor P(x))\land (x \notin B \lor P(x))\Big) \equiv \forall x \in (A\cup B)P(x)$. (distribute over conjunction)

$\forall x\Big(\Big(x \notin A \land x \notin B\Big)\lor P(x)\Big) \equiv \forall x \in (A\cup B)P(x)$. (distribute law)

$\forall x\Big(\neg\Big(x \in A \lor x \in B\Big)\lor P(x)\Big) \equiv \forall x \in (A\cup B)P(x)$. (DeMorgan's law)

$\forall x\Big(\neg\Big(x \in (A \cup B)\Big)\lor P(x)\Big) \equiv \forall x \in (A\cup B)P(x)$. (Definition of $\cup$)

$\forall x\Big(x \in (A \cup B)\implies P(x)\Big) \equiv \forall x \in (A\cup B)P(x)$. (Definition of $\implies$)

$\forall x\in (A \cup B) P(x) \equiv \forall x \in (A\cup B)P(x)$. (abbreviate)

#### 9. Is $\forall x(P(x) \lor Q(x))$ equivalent to $\forall x P(x) \lor \forall xQ(x)$? Explain. (Hint: Try assigning meanings to $P(x)$ and $Q(x)$.)

Let $P(x)$ be "x flag has the color red", and $Q(x)$ be "$x$ flag has the color blue", then our statements become

(i) $\forall x(P(x) \lor Q(x))=$ all flags have either the color red or the color blue

(ii) $\forall x P(x) \lor \forall xQ(x)=$ Either all flags have the color red, or all flags have the color blue

The two statements suggest very different things: (i) says that any flag can have any one of the colors red or blue, or both, so long as they have one, while (ii) is an absolute statement about all the flags: they all have red, or they all have blue.


#### 10.

**(a)** Show that $\exists x \in A P(x) \lor \exists x \in B P(x)$ is equivalent to $\exists x \in (A \cup B) P(x)$.

$\exists x \in A P(x) \lor \exists x \in B P(x) \equiv \exists x \in (A \cup B) P(x)$.

$\exists x \big(x\in A \implies P(x)\big) \lor \exists x \big(x\in B \implies P(x)\big) \equiv \exists x \in (A \cup B) P(x)$ (expand)

$\exists x \neg\big(x\in A \land \neg P(x)\big) \lor \exists x \neg\big(x\in B \land \neg P(x)\big) \equiv \exists x \in (A \cup B) P(x)$ (conditional law)

Since the existential quantifier distributes over disjunction (see exercise 6)

$\exists x\Big[ \neg\big(x\in A \land \neg P(x)\big) \lor \neg\big(x\in B \land \neg P(x)\big)\Big] \equiv \exists x \in (A \cup B) P(x)$ ($\exists$ disjunction distribution)

$\exists x \neg\Big[ \big(x\in A \land \neg P(x)\big) \land \big(x\in B \land \neg P(x)\big)\Big] \equiv \exists x \in (A \cup B) P(x)$ (DeMorgan's law)

$\exists x \neg\Big[ \big(x\notin A \lor  P(x)\big) \land \big(x\notin B \lor P(x)\big)\Big] \equiv \exists x \in (A \cup B) P(x)$ (DeMorgan's law)

$\exists x \neg\Big[ P(x) \lor \big(x\notin A \land x\notin B\big)\Big] \equiv \exists x \in (A \cup B) P(x)$ (Distribuitve property)

$\exists x \neg\Big[ P(x) \lor \neg (x\in A \lor x \in B)\Big] \equiv \exists x \in (A \cup B) P(x)$ (DeMorgan's law)

$\exists x \neg\Big[ P(x) \lor \neg (x\in A \cup B)\Big] \equiv \exists x \in (A \cup B) P(x)$ (union definition)

$\exists x \Big[ \neg P(x) \land x\in A \cup B\Big] \equiv \exists x \in (A \cup B) P(x)$ (DeMorgan's)

Change $\neg P(x) \land x \in A \cup B$ for its Demorgan's equivalent

$\exists x \Big[ P(x) \lor x\notin A \cup B\Big] \equiv \exists x \in (A \cup B) P(x)$ (DeMorgan's)

$\exists x \Big[ x\notin A \cup B \lor P(x)\Big] \equiv \exists x \in (A \cup B) P(x)$ (reordering)

$\exists x \Big[ x\in A \cup B \implies P(x)\Big] \equiv \exists x \in (A \cup B) P(x)$ (conditional law)

$\exists x \in (A \cup B) P(x) \equiv \exists x \in (A \cup B) P(x)$ (abbreviate)

(b) Is $\exists x \in A P(x) \land \exists x \in B P(x)$ equivalent to $\exists x \in (A \cap B) P(x)$?

No, because the two terms in $\exists x \in A P(x) \land \exists x \in B P(x)$ could refer to different entities. It suffices to change the bound variable in one of the terms to see it:

$\exists x \in A P(x) \land \exists y \in B P(y)$

#### \*11 Show that the statements $A \subseteq B$ and $A \setminus B=\varnothing$ are equivalent by writing each in logical symbols then showing that the resulting formulas are equivalent.

$A \subseteq B \equiv A \setminus B = \varnothing$

$\forall x (x \in A \longrightarrow x \in B) \qquad \equiv \qquad \forall x (x \in A \land x \notin B) = \varnothing$

$\forall x (x \notin A \lor x \in B) \qquad \equiv \qquad \forall x (x \in A \land x \notin B) = \varnothing$

Changing the term $x \notin A \lor x \in B$ for its DeMorgan equivalent, we get

$\forall x (x \in A \land x \notin B) \qquad \equiv \qquad \forall x (x \in A \land x \notin B) = \varnothing$


#### 12. Show that the statements $C \subseteq A \cup B$ and $C \setminus A \subseteq B$ are equivalent by writing each in logical symbols and then showing that the resulting formulas are equivalent.

$C \subseteq A \cup B \qquad \equiv \qquad C \setminus A \subseteq B$

$\forall x(x \in C \longrightarrow x\in A \cup B) \qquad \equiv \qquad \forall x (x \in C \setminus A \longrightarrow x\in B)$

$\forall x(x \notin C \lor (x \in A \lor x \in B)) \qquad \equiv \qquad \forall x (\neg(x \in C \land x \notin A) \lor x\in B)$

$\forall x(x \notin C \lor (x \in A \lor x \in B)) \qquad \equiv \qquad \forall x ((x \notin C \lor x \in A) \lor x\in B)$

$\forall x(x \notin C \lor x \in A \lor x \in B) \qquad \equiv \qquad \forall x (x \notin C \lor x \in A \lor x\in B)$

#### 13.

**(a)** Show that the statementsn $A \subseteq B$ and $A \cup B = B$ are equivalent by writing each in logical symbols and then showing that the resulting formulas are equivalent. (Hint: You may find exercise 11 from Section 1.5 useful.)

$A \subseteq B \qquad \equiv \qquad A \cup B$

$\forall x(x \in A \longrightarrow x \in B) \qquad \equiv \qquad \forall x (x \in A \lor x \in B)$

$\forall x(x \notin A \lor x \in B) \qquad \equiv \qquad \forall x (x \in A \lor x \in B)$

Whether $x$ is found in $A$ or not is irrelevant, as long as $x \in B$, the result
 will be equal to $B$.

**(b)** Show that the statements $A \subseteq B$ and $A \cap B$ are equivalent.

$A \subseteq B \qquad \equiv \qquad A \cap B$

$\forall x(x \in A \longrightarrow x\in B) \qquad \equiv \qquad \forall x(x \in A \land x \in B)$

$\forall x(x \notin A \lor x\in B) \qquad \equiv \qquad \forall x(x \in A \land x \in B)$
