---
header-includes:
  - \usepackage{mathrsfs}
---

# Chapter 2.3

#### \*1. Analyze the logical forms of the following statements. You may use the symbols $\in$, $\notin$, $=$, $\neq$, $\land$, $\lor$, $\longrightarrow$, $\iff$, $\forall$ and $\exists$ in your answers, but not $\subseteq$, $\nsubseteq$, $\mathscr{P}$, $\cap$, $\cup$, $\setminus$, $\{$, $\}$, or $\neg$. (Thus, you must write out the definitions of some set theory notation, and you must use equivalences to get rid of any occurrences of ¬.)

- (a) $\mathcal{F}\subseteq\mathscr{P}(A)$.

  By the definition of the subset, every element of $\mathcal{F}$ is also an element of $\mathscr{P}(A)$, then

  $\forall x(x \in \mathcal{F} \longrightarrow x\in \mathscr{P}(A))$

  Rewriting $x \in \mathscr{P}(A)$ as $x \subseteq A$

  $\forall x(x \in \mathcal{F} \longrightarrow x \subseteq A)$

  $\forall x(x \in \mathcal{F} \longrightarrow \forall y(y\in x \longrightarrow y \in A))$

- (b) $A\subseteq\{2n + 1 \mid n \in \mathbb{N}\}$.

  $\forall x(x \in A \longrightarrow x \in \{2n+1 \mid n \in N\})$

  $\forall x(x \in A \longrightarrow \exists n \in \mathbb{N}(x = 2n+1))$

- (c) $\{n^2+n+1 \mid n \in \mathbb{N}\}\subseteq \{2n + 1 \mid n \in \mathbb{N}\}$.

  $\forall n\Big(\{n^2+n+1 \mid n \in \mathbb{N}\} \longrightarrow \{2n + 1 \mid n \in \mathbb{N}\}\Big)$

  $\forall n\Big(\exists m \in \mathbb{N}(\{n^2+n+1 \mid n \in \mathbb{N}\} \longrightarrow \{2n + 1 \mid n \in \mathbb{N}\}\Big)$

  $\exists n \in \mathbb{N}\exists m\in\mathbb{N}(n^2+n+1=2m+1)$

- (d) $\mathscr{P}(\cup_{i\in I}A_i)\nsubseteq\cup_{i\in I}\mathscr{P}(A_i)$.

  Solution:
  <span style="color: #ffff00;">
  $\exists x(\forall y(y\in x \longrightarrow \exists i \in I(y \in A_i))\land \forall i \in I\exists y(y \in x \land y \notin A_i))$
  </span>

  Quoting example 2.3.6: to say that one set is not a subset of another means that there is something that is an element of the first but not the second.

  $\exists x\Bigg(x \in \mathscr{P}(\cup_{i\in I}A_i)\land x\notin\cup_{i\in I}\mathscr{P}(A_i)\Bigg)$

  $\exists x\Bigg(\forall y\Big(y\in x \longrightarrow y\in \cup_{i\in I}A_i\Big)\land \neg \Big(x\in\cup_{i\in I}\mathscr{P}(A_i)\Big)\Bigg)$

  $\exists x\Bigg(\forall y\Big(y\in x \longrightarrow \exists i\in I(y\in A_i)\Big)\land \neg \Big(\exists i \in I (x \subseteq A_i)\Big)\Bigg)$

  $\exists x\Bigg(\forall y\Big(y\in x \longrightarrow \exists i\in I(y\in A_i)\Big)\land \forall i \in I \neg\forall y(y \in x \longrightarrow y \in A_i)\Bigg)$

  $\exists x\Bigg(\forall y\Big(y\in x \longrightarrow \exists i\in I(y\in A_i)\Big)\land \forall i \in I \exists y\neg(y \notin x \lor y \in A_i)\Bigg)$

  $\exists x\Bigg(\forall y\Big(y\in x \longrightarrow \exists i\in I(y\in A_i)\Big)\land \forall i \in I \exists y(y \in x \land y \notin A_i)\Bigg)$

#### 2. Analyze the logical forms of the following statements. You may use the symbols $\in$, $\notin$, $=$, $\neq$, $\land$, $\lor$, $\longrightarrow$, $\iff$, $\forall$ and $\exists$ in your answers, but not $\subseteq$, $\nsubseteq$, $\mathscr{P}$, $\cap$, $\cup$, $\setminus$, $\{$, $\}$, or $\neg$. (Thus, you must write out the definitions of some set theory notation, and you must use equivalences to get rid of any occurrences of ¬.)

- (a) $x \in \cup\mathcal{F}\setminus\cup\mathcal{G}$.

  $x \in \cup \mathcal{F} \land \neg(x \in \cup \mathcal{G})$ (definition of $\setminus$)

  $\exists A(A\in \mathcal{F} \land x \in A) \land \neg(\exists A ( A\in \mathcal{G}\land x \in A))$ (definition of $\cup\mathcal{F}$)

  $\exists A(A\in \mathcal{F} \land x \in A) \land \forall A \neg(A \in \mathcal{G}\land x \in A)$ (quantifier negation)

  $\exists A(A\in \mathcal{F} \land x \in A) \land \forall A (A \notin \mathcal{G}\lor x \notin A)$ (DeMorgan's law)

- (b) $\{x \in B \mid x \notin C \} \in \mathscr{P}(A)$.

  $\exists x(x \in B \land x \notin C ) \subseteq A$

  $\forall y\Big(y \in \exists x(x \in B \land x \notin C ) \longrightarrow y\in A\Big)$

- (c) $x \in \cap_{i\in I}(A_i \cup B_i)$.

* (d) $x \in (\cap_{i\in I}A_i)\cup(\cap_{i\in I}B_i)$.
