### \*1. This problem could be solved by using truth tables, but don't do it that way. Instead, use the methods for writing proofs discussed so far in this chapter. (See Example 3.2.4.)

- (a) Suppose $P \implies Q$ and $Q \implies R$ are both true. Prove that $P \implies R$ is true.

  | Givens         | Goal           |
  | :------------- | :------------- |
  | $P \implies Q$ | $P \implies R$ |
  | $Q \implies R$ |                |

  Since the goal is of the form $P\implies R$, we assume the antecedent and set the consequent as our new goal

  | Givens         | Goal |
  | :------------- | :--- |
  | $P \implies Q$ | $R$  |
  | $Q \implies R$ |      |
  | $P$            |      |

  The proof template looks as such:

  Suppose $P$<br>
  &nbsp;&nbsp;&nbsp;&nbsp;[Proof of R goes here.]<br>
  Therefore, $P\implies R$

  Since we now know $P$, by _modus ponens_ we can infer $Q$. We then add it to the list of givens

  | Givens         | Goal |
  | :------------- | :--- |
  | $P \implies Q$ | $R$  |
  | $Q \implies R$ |      |
  | $P$            |      |
  | $Q$            |      |

  Then, our proof template looks as below:

  Suppose $P$<br>
  &nbsp;&nbsp;&nbsp;&nbsp;Suppose Q<br>
  &nbsp;&nbsp;&nbsp;&nbsp;&nbsp;&nbsp;&nbsp;&nbsp;[Proof of R goes here.]<br>
  &nbsp;&nbsp;&nbsp;&nbsp;Therefore, $P\implies Q$<br>
  Therefore, $P\implies R$

  Since we now know $Q$, by _modus ponens_ we can infer $R$. The proof is done.

  **Theorem.** _Suppose $P \implies Q$ and $Q \implies R$. Then $P \implies R$._

  _Proof._ Suppose $P \implies Q$, $Q \implies R$ and $P$. Since $P$ and $P \implies Q$, it follows that $Q$. Then, since $Q$ and $Q \implies R$, we can conclude that $R$. Therefore, $P \implies R$. $\square$

- (b) Suppose $\neg R \implies (P \implies \neg Q)$ is true. Prove that $P \implies (Q \implies R)$ is true.

  | Givens                                | Goal                        |
  | :------------------------------------ | :-------------------------- |
  | $\neg R \implies (P \implies \neg Q)$ | $P \implies (Q \implies R)$ |

  We can start by assuming that the goal antecedent is true. Then our givens are

  | Givens                                | Goal           |
  | :------------------------------------ | :------------- |
  | $\neg R \implies (P \implies \neg Q)$ | $Q \implies R$ |
  | $P$                                   |                |

  And our proof template has the form:

  Suppose $P$<br>
  &nbsp;&nbsp;&nbsp;&nbsp;[Proof of $Q\implies R$ goes here.]<br>
  Therefore, $P \implies (Q \implies R)$

  Iterating on the same strategy once more, as the new goal is another conditional

  | Givens                                | Goal |
  | :------------------------------------ | :--- |
  | $\neg R \implies (P \implies \neg Q)$ | $R$  |
  | $P$                                   |      |
  | $Q$                                   |      |

  Template:

  Suppose $P$<br>
  &nbsp;&nbsp;&nbsp;&nbsp;Suppose $Q$<br>
  &nbsp;&nbsp;&nbsp;&nbsp;&nbsp;&nbsp;&nbsp;&nbsp;[Proof of $R$ goes here.]<br>
  &nbsp;&nbsp;&nbsp;&nbsp;Therefore, $Q \implies R$<br>
  Therefore, $P \implies (Q \implies R)$

  Since we now know $P \implies Q$ is true, then $P \implies \neg Q$ is false. Thus, since $\neg R \implies (P \implies \neg Q)$ is true, by _modus tollens_ we can conclude that $\neg R$ must also be false. Therefore, $R$ is true.

  **Theorem.** _Suppose $\neg R \implies (P \implies \neg Q)$ is true. Prove that $P \implies (Q \implies R)$ is true._

  _Proof._ Suppose $P$, $Q$ and $\neg R \implies (P \implies \neg Q)$. Since $P$ and $Q$, $P \implies Q$ is true, which means $P \implies \neg Q$ is false. By _modus tollens_ we can conclude that $\neg R$ must also be false, which in turn means $R$ is true. Since $P$, $Q$ and $R$ are true, $P \implies (Q \implies R)$ is true. Therefore, if $\neg R \implies (P \implies \neg Q)$, then $P \implies (Q \implies R)$. $\square$

### 2. This problem could be solved by using truth tables, but don't do it that way. Instead, use the methods for writing proofs discussed so far in this chapter. (See Example 3.2.4.)

- (a) Suppose $P \implies Q$ and $R \implies \neg Q$ are both true. Prove that $P \implies \neg R$ is true.

  | Givens              | Goal                |
  | :------------------ | :------------------ |
  | $P \implies Q$      | $P \implies \neg R$ |
  | $R \implies \neg Q$ |                     |

  Suppose $P$, then

  | Givens              | Goal     |
  | :------------------ | :------- |
  | $P \implies Q$      | $\neg R$ |
  | $R \implies \neg Q$ |          |
  | $P$                 |          |

  Since $P$ and $P \implies Q$, by _modus ponens_ we can conclude that $Q$ is true. Then, since we know $Q$ and $R \implies \neg Q$, we can conclude (by _modus tollens_) that $R$ is false, thus, $\neg R$ is true.

  **Theorem.** _Suppose $P \implies Q$ and $R \implies \neg Q$ are both true. Prove that $P \implies \neg R$ is true._

  _Proof._ Suppose $P$, since $P$ and $P \implies Q$, we can infer $Q$, then, since $Q$ and $R \implies \neg Q$, we can conclude $R$ is false, thus $\neg R$ is true. Therefore, if $P \implies Q$ and $R \implies \neg Q$, then $P \implies \neg R$. $\square$

* (b) Suppose that $P$ is true. Prove that $Q \implies \neg (Q \implies \neg P)$ is true.

  Rewriting $\neg (Q \implies \neg P)$, we have

  $\neg (\neg Q \lor \neg P) \equiv Q \land P$

  Then

  | Givens | Goal                   |
  | :----- | :--------------------- |
  | $P$    | $Q \implies Q \land P$ |

  Suppose $Q$, then

  | Givens | Goal        |
  | :----- | :---------- |
  | $P$    | $Q \land P$ |
  | $Q$    |             |

  **Theorem.** _Suppose that $P$ is true. Prove that $Q \implies \neg (Q \implies \neg P)$ is true._

  _Proof._ Suppose $Q$. By rewriting $Q \implies \neg (Q \implies \neg P)$ as it's equivalent $Q \implies Q \land P$, given $Q$ and $P$, we can conclude that, if $P$, then $Q \implies \neg (Q \implies \neg P)$. $\square$

### 3. Suppose $A \subseteq C$, and $B$ and $C$ are disjoint. Prove that if $x \in A$ then $x \notin B$.

$B$ and $C$ being disjoint means that $B \cap C=\varnothing$. This also means that $B \setminus C=B$. Then we have

| Givens                 | Goal                          |
| :--------------------- | :---------------------------- |
| $A \subseteq C$        | $x \in A \implies x \notin B$ |
| $B \cap C=\varnothing$ |                               |

Assume $x \in A$, then

| Givens                 | Goal         |
| :--------------------- | :----------- |
| $A \subseteq C$        | $x \notin B$ |
| $B \cap C=\varnothing$ |              |
| $x \in A$              |              |

Since $x \in A$ and $A \subseteq C$, it follows that $x \in C$. Now, since $B \cap C=\varnothing$, it follows that $x \notin B$. Therefore, if $x \in A$, then $x \notin B$

### 4. Suppose that $A \setminus B$ is disjoint from $C$ and $x \in A$. Prove that if $x \in C$ then $x \in B$.

| Givens                             | Goal                      |
| :--------------------------------- | :------------------------ |
| $A \setminus B \cap C=\varnothing$ | $x\in C \implies x \in B$ |
| $x \in A$                          |                           |

Assume $x \in C$, then

| Givens                              | Goal      |
| :---------------------------------- | :-------- |
| $(A \setminus B)\cap C=\varnothing$ | $x \in B$ |
| $x \in A$                           |           |
| $x \in C$                           |           |

Suppose $x \in C$, since $(A \setminus B) \cap C=\varnothing$, it follows that $x \notin A\setminus B$. Then, $x \notin A\setminus B\equiv \neg(x \in A \land x \notin B)\equiv x\notin A \lor x \in B$. Since $x \in A$, it follows that $x \in B$. Therefore, if $x\in A$, then $x \in B$.

### 5. Use the method of proof by contradiction to prove the theorem in Example 3.2.1.

**Theorem.** Suppose $A \cap C \subseteq B$ and $a \in C$. Then $a\notin A \setminus B$.

By contradiction. Assume $a \in A \setminus B \equiv (a \in A \land a \notin B)$. Since $a \in C$, then $a \in A \cap C \subseteq B$, thus it follows that $a \in B$. This contradicts the fact that $a \notin B$, therefore, $a \notin A \setminus B$.

### 6. Use the method of proof by contradiction to prove the theorem in Example 3.2.5.

**Theorem.** Suppose that $A \subseteq B$, $a \in A$, and $a \notin B \setminus C$. Then $a \in C$.

| Givens                   | Goal      |
| :----------------------- | :-------- |
| $A \subseteq B$          | $a \in C$ |
| $a \in A$                |           |
| $a \notin B \setminus C$ |           |

Suppose $a \notin C$. Given $x \in A$, and $A \subseteq B$, it follows that $a \in B$. Since $a \in B$, and $a \notin C$, it follows that $a \in B \setminus C$, but this contradicts the fact that $a \notin B \setminus C$. Therefore, $a \in C$.

#### 7. Suppose that $y + x = 2y − x$, and $x$ and $y$ are not both zero. Prove that $y \neq 0$.

_Proof._ By contradiction. Assume $y = 0$, then, it follows from $(0) + x = 2(0) - x$ that $x = 0$. Since $y = 0$, and $x = 0$, this contradicts the fact that $x$ and $y$ are not both $0$. Therefore, $y \neq 0$.

### \*8. Suppose that $a$ and $b$ are nonzero real numbers. Prove that if $a \lt \frac{1}{a} \lt b \lt \frac{1}{b}$ then $a \lt -1$.

Assume $a \lt \frac{1}{a} \lt b \lt \frac{1}{b}$.

Since $a \lt \frac{1}{a}$, then $a \in (-\infty, -1) \lor (0,1)$, likewise $b \lt \frac{1}{b}$, then $b \in (-\infty, -1) \lor (0,1)$

Leading to four cases to analyze:

1. $a \in (-\infty, -1)$ and $b\in (-infty, -1)$. Since $a$ and $b$ share the same sign, and $\frac{1}{a} \lt \frac{1}{b}$, then $a \gt b$, but this contradicts the fact that $a \lt b$. Not possible.

2. $a \in (-\infty, -1)$ and $b\in (0,1)$. Here, $a$ is negative and $b$ is not, therefore $\frac{1}{a} \lt \frac{1}{b}$ implies $a \lt b$.

3. $a \in (0,1)$ and $b\in (-infty, -1)$. Here, $b$ is negative and $a$ is not. This is a contradiction of the fact that $a \lt b$.

4. $a \in (0,1)$ and $b \in (0,1)$, Here both $a$ and $b$ are positive and in the $(0,1)$ range. This implies that $\frac{1}{a}\gt 1$, this cannot be as $\frac{1}{a}\lt b$ and $b\lt 1$

Since case 2 is true, it follows that $a \lt -1$.

### 9. Suppose that $x$ and $y$ are real numbers. Prove that if $x^2y=2x+y$, then if $y \neq 0$ then $x\neq0$.

| Givens      | Goal                         |
| :---------- | :--------------------------- |
| $x^2y=2x+y$ | $y \neq 0 \implies x \neq 0$ |

Assume $y \neq 0$, then

| Givens      | Goal       |
| :---------- | :--------- |
| $x^2y=2x+y$ | $x \neq 0$ |
| $y \neq 0$  |            |

Assume the contrary, that $x = 0$, then

| Givens      | Goal          |
| :---------- | :------------ |
| $x^2y=2x+y$ | Contradiction |
| $y \neq 0$  |               |
| $x = 0$     |               |

**Theorem**. If $x^2y = 2x+y$, then if $y \neq 0$ then $x \neq 0$.

_Proof_. By contradiction.<br>
Suppose $x^2y=2x+y$ and $y \neq 0$<br>
&nbsp;&nbsp;&nbsp;&nbsp;Suppose $x=0$<br>
&nbsp;&nbsp;&nbsp;&nbsp;&nbsp;&nbsp;&nbsp;&nbsp;Then $x^2y=2x+y$ becomes $0=y$, but this contradicts the fact that $y\neq 0$.<br>
&nbsp;&nbsp;&nbsp;&nbsp;Therefore $x \neq 0$<br>
Thus, if $x^2y=2x+y$ and $y \neq 0$, then $x \neq 0$

### 10. Suppose that $x$ and $y$ are real numbers. Prove that if $x \neq 0$, then if $y = \frac{3x^2+2y}{x^2+2}$ then $y = 3$.

Simplifying $y = \frac{3x^2+2y}{x^2+2}$ yields

$y = \frac{3x^2+2y}{x^2+2}$

$x^2y -3x^2 = 0$

$(y-3)x^2 = 0$

Suppose $x \neq 0$, and $(y-3)x^2=0$. It follows that $y-3=0$, therefore, $y=3$. Thus, $x \neq 0 \implies (y = \frac{3x^2+2y}{x^2+2} \implies y=3)$

### \*11. Consider the following incorrect theorem:

**Incorrect Theorem.** Suppose $x$ and $y$ are real numbers and $x+y=10$. Then $x\neq 3$ and $y \neq 8$.

- (a) What's wrong with the following proof of the theorem?

  _Proof._ Suppose the conclusion of the theorem is false. Then $x = 3$ and $y = 8$. But then $x + y = 11$, which contradicts the given information that $x + y = 10$. Therefore the conclusion must be true.

  Just assuming the theorem is false does not mean $x=3$ and $y=8$.

  They assume

  $\neg \Big(x+y=10 \implies x \neq 3 \land y \neq 8\Big)$

  But the right side of the implication becomes

  $x = 3 \lor y = 8$ by DeMorgan's

- (b) Show that the theorem is incorrect by finding a counterexample.

  Two counterexamples exist: $x=3$ and $y=7$, and $x=2$ and $y=8$.

### 12. Consider the following incorrect theorem:

**Incorrect Theorem**. Suppose that $A \subseteq C$, $B \subseteq C$, and $x \in A$. Then $x \in B$.

- (a) What’s wrong with the following proof of the theorem?

  _Proof._ Suppose that $x \notin B$. Since $x \in A$ and $A \subseteq C$, $x\in C$. Since $x \notin B$ and $B\subseteq C$, $x \notin C$. But now we have proven both $x \in C$ and $x \notin C$, so we have reached a contradiction. Therefore $x \in B$.

  The statement $x \notin B$ and $B\subseteq C$, $x \notin C$ is incorrect.$x \notin B$ and $B\subseteq C$ do not impli $x \notin C$.

- (b) Show that the theorem is incorrect by finding a counterexample.

### 13. Use truth tables to show that modus tollens is a valid rule of inference.

|                $P$                 |                $Q$                 |           $P \implies Q$           |
| :--------------------------------: | :--------------------------------: | :--------------------------------: |
|                 T                  |                 T                  |                 T                  |
| <span style="color: red;">T</span> | <span style="color: red;">F</span> | <span style="color: red;">T</span> |
|                 F                  |                 T                  |                 F                  |
|                 F                  |                 F                  |                 T                  |

### \*14. Use truth tables to check the correctness of the theorem in Example 3.2.4.

Recall Example 3.2.4:

Suppose $P \implies (Q \implies R)$. Prove that $\neg R \implies (P \implies \neg Q)$.

| No. | $P$ | $Q$ | $R$ | $Q \implies R$ | $P \implies (Q \implies R)$ | $P \implies \neg Q$ | $\neg R \implies (P \implies \neg Q)$ |
| :-: | :-: | :-: | :-: | :------------: | :-------------------------: | :-----------------: | :-----------------------------------: |
|  1  |  F  |  F  |  F  |       T        |              T              |          T          |                   T                   |
|  2  |  F  |  F  |  T  |       T        |              T              |          T          |                   T                   |
|  3  |  F  |  T  |  F  |       T        |              T              |          T          |                   T                   |
|  4  |  F  |  T  |  T  |       T        |              T              |          T          |                   T                   |
|  5  |  T  |  F  |  F  |       T        |              T              |          T          |                   T                   |
|  6  |  T  |  F  |  T  |       T        |              T              |          T          |                   T                   |
|  7  |  T  |  T  |  F  |       F        |              F              |          F          |                   F                   |
|  8  |  T  |  T  |  T  |       T        |              T              |          F          |                   T                   |

Lines 4, 6 and 8 prove it as true.

### 17. Can the proof in Example 3.2.2 be modified to prove that if $x^2 + y = 13$ and $x \neq 3$ then $y \neq 4$? Explain.

Recall example 3.2.2's theorem:

**Theorem 3.2.2**. If $x^2 + y = 13$ and $y \neq 4$ then $x \neq 3$.

No. To do that you would have to do the contrapositive, then work your way up to those statements.

We can represent it as:

$\Big((x^2 + y = 13) \land y \neq 4 \Big)\implies x \neq 3$.

Which becomes (by contrapositive)

$x = 3 \implies \neg\Big((x^2 + y = 13) \land y \neq 4 \Big)$.

$x = 3 \implies \Big(x^2 + y \neq 13 \lor y = 4 \Big)$.

Leaving the inverted form as

$x = 3 \implies \Big(x^2 + y = 13 \implies y = 4 \Big)$.

| Givens  | Goal                          |
| :------ | :---------------------------- |
| $x = 3$ | $x^2 + y = 13 \implies y = 4$ |

We then assume $x^2 + y = 13$, and have

| Givens         | Goal    |
| :------------- | :------ |
| $x = 3$        | $y = 4$ |
| $x^2 + y = 13$ |         |

Which then becomes trivial to prove, since $x = 3$, substitute into $x^2+y=13$ and get $y=4$.

Swapping out the conditionals as suggested would have changed the correctness of the theorem (and the proof).
