### \*1. In exercise 7 of Section 2.2 you used logical equivalences to show that $\exists x \Big(P(x) \implies Q(x)\Big)$ is equivalent to $\forall x P(x) \implies \exists x Q(x)$. Now use the methods of this section to prove that if $\exist x \Big(P(x) \implies Q(x)\Big)$ is true, then $\forall x P(x) \implies \exists x Q(x)$ is true. (Note: The other direction of the equivalence is quite a bit harder to prove. See exercise 29 of Section 3.5.)

| Givens                         | Goal                                    |
| :----------------------------- | :-------------------------------------- |
| $\exist x(P(x) \implies Q(x))$ | $\forall x P(x) \implies \exist x Q(x)$ |

By existential instantiation, assume $x_0$ such that $P(x_0)$ is true, then

| Givens                   | Goal                                    |
| :----------------------- | :-------------------------------------- |
| $P(x_0) \implies Q(x_0)$ | $\forall x P(x) \implies \exist x Q(x)$ |

Let $x$ be arbitrary, then assume $P(x)$

| Givens                   | Goal            |
| :----------------------- | :-------------- |
| $P(x_0) \implies Q(x_0)$ | $\exist x Q(x)$ |
| P(x)                     |                 |

Since $P(x)$, we know $P(x_0)$ is true and $P(x_0) \implies Q(x_0)$, by modus ponens we know $Q(x_0)$ is true. Therefore, $\exist x Q(x)$.

**Theorem.** If $\exist x(P(x) \implies Q(x))$, then $\forall x P(x) \implies \exist x Q(x)$.

_Proof._ Since we know $\exist x(P(x) \implies Q(x))$, let $x_0$ be an element such that $P(x_0) \implies Q(x_0)$. Let $x$ be arbitrary, and assume $P(x)$. since $P(x)$ is true, so is $P(x_0)$, then, by modus ponens, we can determine $Q(x)$ is true. Therefore, If $\exist x(P(x) \implies Q(x))$, then $\forall x P(x) \implies \exist x Q(x)$. $\square$

### 2. Prove that if $A$ and $B \setminus C$ are disjoint, $A \cap B \subseteq C$.

| Givens                                 | Goal                                        |
| :------------------------------------- | :------------------------------------------ |
| $A \cap (B \setminus C) = \varnothing$ | $\forall x(x\in A \cap B \implies x \in C)$ |

Let x be arbitrary, and assume $x \in A\cap B$, then

| Givens                                 | Goal      |
| :------------------------------------- | :-------- |
| $A \cap (B \setminus C) = \varnothing$ | $x \in C$ |
| $x\in A \cap B$                        |           |

Since $x \in A \cap B = (x\in A \land x\in B)$

| Givens                                 | Goal      |
| :------------------------------------- | :-------- |
| $A \cap (B \setminus C) = \varnothing$ | $x \in C$ |
| $x\in A$                               |           |
| $x\in B$                               |           |

**Theorem**. If $A \cap B \setminus C =\varnothing$, then $A \cap B \subseteq C$.

_Proof_. Let $x$ be arbitrary, suppose $A \cap (B\setminus C)=\varnothing$ and suppose $x \in A\cap B$. Since $x\in A \cap B$, $x\in B$ and $x\in A$. Since $x$ was arbitrary, and given $A \cap (B\setminus C)=\varnothing$, we can conclude that $A \cap B \subseteq C$.

### \*3. Prove that if $A \subseteq B \setminus C$ then $A$ and $C$ are disjoint.

Assume, to the contrary, that $A$ and $C$ are not disjoint.

Then we can choose some $x$, call it $x_0$, by universal instantiation such that $x_0 \in A$ and $x_0 \in C$.

Since we know $x_0 \in A$, and since $\forall x(x \in A \implies x\in B \setminus C)$, then $x_0 \in A \implies x_0\in B \land x_0 \notin C$

But now we have $x_0 \in C$ and $x_0 \notin C$, which is a contradiction. Therefore, $A$ and $C$ must be disjoint.

### 4. Suppose $A \subseteq \mathscr{P}(A)$. Prove that $\mathscr{P}(A) \subseteq \mathscr{P} ( \mathscr{P}(A))$.

Suppose $x \in \mathscr{P}(A)$. Then $x \subseteq A$. Since it is given that $A \subseteq \mathscr{P}(A)$, it follows that $x \subseteq \mathscr{P}(A)$. Thus if $x \in \mathscr{P}(A)$, then $x \in \mathscr{P}( \mathscr{P}(A))$. As $x$ is arbitrary, we get $\mathscr{P}(A) \subseteq \mathscr{P}( \mathscr{P}(A))$.

### 5. The hypothesis proven in exercise 4 is $A \subseteq \mathscr{P}(A)$.

- (a) Can you think of a set $A$ for which this hypothesis is true?

  $\varnothing$, the empty set.

- (b) Can you think of another?

  no such set exists besides $\varnothing$

### 6. Suppose $x$ is a real number.

- (a) Prove that if $x \neq 1$, then there is a number $y$ such that $\frac{y+1}{y-2}=x$.

| Givens    | Goal                                  |
| :-------- | :------------------------------------ |
| $x\neq 1$ | $\exist y\Big(\frac{y+1}{y-2}=x\Big)$ |

$$y+1-xy +2x=0$$
$$y(1-x)=-2x-1$$
$$y=\frac{2x+1}{x-1}$$

Suppose $y=\frac{2x+1}{x-1}$, then, plugging in this value in the equation

$$x=\frac{\frac{2x+1}{x-1}+1}{\frac{2x+1}{x-1}-2}$$
$$x=\frac{\frac{2x+1+x-1}{x-1}}{\frac{2x+1-2x+2}{x-1}}$$
$$x=\frac{\frac{3x}{x-1}}{\frac{3}{x-1}}$$
$$x=\frac{3x}{x-1} \times\frac{x-1}{3}$$
$$x=\frac{\sout{3}x}{\sout{x-1}} \times\frac{\sout{x-1}}{\sout{3}}$$
$$x=x$$

- (b) Prove that if there is a real number $y$ such that $\frac{y+1}{y-2}=x$, then $x \neq 1$.

Given $y=\frac{2x+1}{x-1}$, we can solve for $y=\frac{2x+1}{x-1}$, given $y \in \R$, so is $\frac{2x+1}{x-1}\in R$, therefore $x-1\neq 0$. Thus, $x \neq 0$.

### \*7. Prove that for every real number $x$, if $x \gt 2$ then there is a real number $y$ such that $y + \frac{1}{y} = x$.

$$ y +\frac{1}{y}=x$$
$$ y^2 - xy+1=0$$

$$y = \frac{x\plusmn\sqrt{x^2-4}}{2}$$

Which is real since $x \gt 2$, means $\sqrt{x^2-4} \in \R$

Since we only need one element to provide proof, we'll take $y = \frac{x+\sqrt{x^2-4}}{2}$.

Substituting into the original definition for $y$:

$$x=\frac{x+\sqrt{x^2-4}}{2}+ \frac{2}{x+\sqrt{x^2-4}}$$
$$x=\frac{(x+\sqrt{x^2-4})^2 + 4}{2(x+\sqrt{x^2-4})}$$
$$x=\frac{x^2+2x\sqrt{x^2-4}+x^2-4 + 4}{2(x+\sqrt{x^2-4})}$$
$$x=\frac{2x^2+2x\sqrt{x^2-4}}{2(x+\sqrt{x^2-4})}$$
$$x=\frac{x^2+x\sqrt{x^2-4}}{x+\sqrt{x^2-4}}$$
$$x=\frac{x(x+\sqrt{x^2-4})}{x+\sqrt{x^2-4}}$$
$$x=x$$

Therefore, $y + \frac{1}{y} = x$.

### 8. Prove that if $\mathcal{F}$ is a family of sets and $A \in \mathcal{F}$, then $A \subseteq \cup \mathcal{F}$.

| Givens              | Goal                                                 |
| :------------------ | :--------------------------------------------------- |
| $A \in \mathcal{F}$ | $\forall x(x \in A \implies x \in \cup \mathcal{F})$ |

| Givens              | Goal                                                                    |
| :------------------ | :---------------------------------------------------------------------- |
| $A \in \mathcal{F}$ | $\forall x\Big(x \in A \implies \exist A \in \mathcal{F}(x\in A) \Big)$ |

Let $x$ be arbitrary, then

| Givens              | Goal                               |
| :------------------ | :--------------------------------- |
| $A \in \mathcal{F}$ | $\exist A \in \mathcal{F}(x\in A)$ |
| $x \in A$           |                                    |

Since $A \in \mathcal{F}$ and $x \in A$. Since $x$ was arbitrary, we can conclude that $A \subseteq \cup \mathcal{F}$.

### \*9. Prove that if $\mathcal{F}$ is a family of sets and $A \in \mathcal{F}$, then $\cap \mathcal{F} \subseteq A$.

| Givens              | Goal                                                 |
| :------------------ | :--------------------------------------------------- |
| $A \in \mathcal{F}$ | $\forall x(x \in \cap \mathcal{F} \implies x \in A)$ |

Let $x$ be arbitrary

| Givens                               | Goal      |
| :----------------------------------- | :-------- |
| $A \in \mathcal{F}$                  | $x \in A$ |
| $\forall A \in \mathcal{F}(x \in A)$ |           |

Given $A \in \mathcal{F}$ and $\forall A \in \mathcal{F}(x \in A)$, since $x$ was arbitrary, we can conclude that $x \in A$. Therefore $\cap \mathcal{F}\subseteq A$.

### 10. Suppose that $\mathcal{F}$ is a nonempty family of sets, $B$ is a set, and $\forall A \in \mathcal{F}(B\subseteq A)$. Prove that $B \subseteq \cap \mathcal{F}$.

Given $\mathcal{F}\neq \varnothing$, $B$, and $\forall A \in \mathcal{F}(\forall x(x \in B \implies x\in A))$, since $B$ is a subset of every set $A$ in $\mathcal{F}$, then at least one element of $B$ is in every set $A$ of $\mathcal{F}$, thus $B \subseteq \cap \mathcal{F}$.

### 11. Supose that $\mathcal{F}$ is a family of sets. Prove that if $\varnothing \subseteq \mathcal{F}$ then $\cap \mathcal{F}=\varnothing$.

Given that $\varnothing \subseteq \mathcal{F}$, which means $\exist A \in \mathcal{F}(\varnothing \in \mathcal{A})$, and the fact that for any set $A$, $A \cap \varnothing = \varnothing$, we can conclude that $\forall A \in \mathcal{F}(x \in A)=\cap \mathcal{F}=\varnothing$

### \*12. Suppose $\mathcal{F}$ and $\mathcal{G}$ are families of sets. Prove that if $\mathcal{F} \subseteq \mathcal{G}$ then $\cup \mathcal{F} \subseteq \cup \mathcal{G}$.

Given

$\mathcal{F} \subseteq \mathcal{G} = \forall x (x \in \mathcal{F} \implies x\in \mathcal{G})$

$\cup \mathcal{F} \subseteq \cup \mathcal{G} =\forall x(x \in \cup \mathcal{F} \implies x \in \cup \mathcal{G})$

Let $x$ be an arbitrary set.

|                          Givens                           |           Goal           |
| :-------------------------------------------------------: | :----------------------: |
| $\forall x (x \in \mathcal{F} \implies x\in \mathcal{G})$ | $x \in \cup \mathcal{G}$ |
|                 $x \in \cup \mathcal{F}$                  |                          |

Rewriting the second given and the goal for their definitions in logical symbols

|                          Givens                           |                  Goal                   |
| :-------------------------------------------------------: | :-------------------------------------: |
| $\forall x (x \in \mathcal{F} \implies x\in \mathcal{G})$ | $\exist A \in \cup\mathcal{G}(x \in A)$ |
|          $\exist A \in \cup\mathcal{F}(x \in A)$          |                                         |

Let $A_0$ be an element of $\mathcal{F}$, then we can plug in $A_0$ in the given using universal instantiation

|                       Givens                       |                  Goal                   |
| :------------------------------------------------: | :-------------------------------------: |
| $A_0 \in \mathcal{F} \implies A_0 \in \mathcal{G}$ | $\exist A \in \cup\mathcal{G}(x \in A)$ |
|             $A_0 \in \cup\mathcal{F}$              |                                         |

Since we know $A_0 \in \cup \mathcal{F}$, which implies $A_0 \in \mathcal{F}$, and $A_0 \in \mathcal{F} \implies A_0 \in \mathcal{G}$, by modus ponens we can conclude that $A_0 \in \mathcal{G}$, therefore $A_0 \in \cup \mathcal{G}$. Thus, $\exist A \in \cup\mathcal{G}(x \in A)$.

**Theorem**. $\mathcal{F}$ and $\mathcal{G}$ are families of sets. If $\mathcal{F} \subseteq \mathcal{G}$ then $\cup \mathcal{F} \subseteq \cup \mathcal{G}$.

_Proof_. Suppose $x \in \cup \mathcal{F}$. We can let $A_0$ be an element of $\cup \mathcal{F}$. Thus, $A_0 \in \mathcal{F}$. Since $\mathcal{F} \subseteq \mathcal{G}$ and $A_0 \in \mathcal{F}$, by modus ponens we can conclude that $A_0 \in \mathcal{G}$, which implies $A_0 \in \cup \mathcal{G}$. Therefore, if $\mathcal{F} \subseteq \mathcal{G}$ then $\cup \mathcal{F} \subseteq \cup \mathcal{G}$.

### 13. Suppose $\mathcal{F}$ and $\mathcal{G}$ are families of sets. Prove that if $\mathcal{F} \subseteq \mathcal{G}$ then $\cap \mathcal{G} \subseteq \cap \mathcal{F}$.

$\mathcal{F} \subseteq \mathcal{G} = \forall A(A\in \mathcal{F} \implies A \in \mathcal{G})$

$\cap \mathcal{G} \subseteq \cap \mathcal{F} = \forall A (A \in \cap \mathcal{G} \implies A \in \cap \mathcal{F})$

Let $x$ be an arbitrary set. Assume $A \in \cap \mathcal{G}$, then $x$ is found in all of the sets of $\mathcal{G}$. Since $\mathcal{F} \subseteq \mathcal{G}$, $x$ must also belong to all the sets of $\mathcal{F}$. Therefore, $x \in \cap \mathcal{G} \subseteq \implies x \in \mathcal.{F}$

### 14. Suppose $\{A_i \mid i \in I\}$ is an indexed family of sets. Prove that $\cup_{i \in I}\mathscr{P}(A_i) \subseteq \mathscr{P}(\cup_{i \in I} A_i)$. (Hint: First make sure you know what al the notation means!)

Break it down:

$$\cup_{i \in I}\mathscr{P}(A_i) \subseteq \mathscr{P}(\cup_{i \in I} A_i)$$

$$\forall x\Big(x \in \cup_{i \in I}\mathscr{P}(A_i) \implies x \in \mathscr{P}(\cup_{i \in I} A_i)\Big)$$

Let $x$ be an arbitrary set, assume $x \in \cup_{i \in I}\mathscr{P}(A_i)$. Suppose $A_0$ is one of the sets in the family $_{i \in I}\mathscr{P}(A_i)$, and $x \in \mathscr{P}(A_0)$, it follows that $x \subseteq A_0$, then $x \subseteq \cup_{i \in I}A_i$. From this, we can conclude that $x \in \mathscr{P}(\cup_{i \in I}A_i)$.
