### \*1. Use the methods of this chapter to prove that $\forall x (P(x) \land Q(x))$ is equivalent to $\forall x P(x) \lor \forall x Q(x)$.

($\rightarrow$) Let $y$ be arbitrary, then since $\forall x (P(x) \land Q(x))$, it follows that $P(y) \land Q(y)$. Since $P(y)$, and since $y$ was arbitrary, it follows that $\forall xP(x)$. Since $Q(y)$, and since $y$ was arbitrary, it follows that $\forall xQ(x)$.

($\leftarrow$) Suppose $\forall x P(x) \lor \forall x Q(x)$, and let $y$ be arbitrary. Since $\forall x P(x)$, then $P(y)$, likewise since $\forall x Q(x)$, then $Q(y)$. Since $P(y)$ and $Q(y)$, and since $y$ was arbitrary, $\forall x(P(x) \land Q(x))$.

### \*4. Prove that if $A \subseteq B$ and $A \nsubseteq C$ then $B \nsubseteq C$.

In logical forms

$A \subseteq B = \forall x(x \in A \implies x \in B)$

$A \nsubseteq C = \neg(\forall x(x \in A \implies x \in C))=\exist x (x \in A \land x \notin C)$

$\exist x (x \in B \land x \notin C)$

| Givens                         | Goals                                 |
| :----------------------------- | :------------------------------------ |
| $x_0 \in A \implies x_0 \in B$ | $\exist x (x \in B \land x \notin C)$ |
| $x_0 \in A$                    |                                       |

| $x_0 \notin C$

Let $x_0$ be an element that satisfies $A \nsubseteq C = \exist x (x \in A \land x \notin C)$. Since we know $x_0 \in A$, and $x_0 \in A \implies x_0 \in B$, by modus ponens we can conclude that $x_0 \in B$, and since $x_0 \notin C$, we can conclude that $\exist x (x \in B \land x \notin C)$. Thus, if $A \subseteq B$ and $A \nsubseteq C$, then $B \nsubseteq C$.
