**Example 1.2.5.** Find simpler formulas equivalent to these formulas:
1. $\neg (P \lor \neg Q)$.
    - Through DeMorgan's law $\neg (P \lor \neg Q) \equiv \neg P \land \neg \neg Q$
    - Then through double negation and commutative $\neg P \land \neg \neg Q \equiv$<span style="color:darkred;">$Q\land \neg P$</span>
2. $\neg (Q \land \neg P) \lor P$.
    - Through DeMorgan's: $\neg (Q \land \neg P) \lor P\equiv(\neg Q \lor \neg \neg P)\lor P$
    - Then through double negation: $(\neg Q \lor \neg \neg P)\lor P \equiv (\neg Q \lor P) \lor P$
    - Through the associative law: $(\neg Q \lor P) \lor P\equiv\neg Q \lor (P \lor P)$
    - Idempotence: $\neg Q \lor (P \lor P)\equiv$<span style="color:darkred">$\neg Q \lor P$</span>
  