#### \*1. Analyze the logical forms of the following statements:

- (a) If this gas either has an unpleasant smell or is not explosive, then it isn’t hydrogen.

  $(S \land \neg E) \longrightarrow \neg H$ where $S$ stands for "has an unpleasant smell", $E$ stands for "it's explosive" and $H$ stands for "it's hydrogen"

- (b) Having both a fever and a headache is a sufficient condition for George to go to the doctor.

  $(F \land H) \longrightarrow D$

- (c) Both having a fever and having a headache are sufficient conditions for George to go to the doctor.

  $(F \longrightarrow D) \lor (H \longrightarrow D)$

- (d) If $x \neq 2$, then a necessary condition for $x$ to be prime is that $x$ be odd.

  $(x \neq 2) \longrightarrow P(x) \longrightarrow O(x)$

#### 2. Analyze the logical forms of the following statements:

- (a) Mary will sell her house only if she can get a good price and find a nice apartment.

  $(G \land N) \longrightarrow S$

- (b) Having both a good credit history and an adequate down payment is a necessary condition for getting a mortgage.

  $(C \land D) \longrightarrow M$

- (c) John will kill himself, unless someone stops him. (Hint: First try to rephrase this using the words if and then instead of unless.)

  Let

  $S$ be "someone stopped John"

  $K$ be "John will kill himself"

  $S \longrightarrow \neg K = K \longrightarrow \neg S$

- (d) If x is divisible by either 4 or 6, then it isn’t prime.

  $D \longrightarrow \neg P$

#### \*4. Use truth tables to determine whether or not the following arguments are valid:

- (a) Either sales or expenses will go up. If sales go up, then the boss will be happy. If expenses go up, then the boss will be unhappy. Therefore, sales and expenses will not both go up.

  Let $S$ be "sales will go up", $E$ be "expenses will go up", $H$ be "the boss will be happy.

  $S \lor E$

  $S \longrightarrow H$

  $E \longrightarrow \neg H$

  $-----$

  $\therefore \neg S \land \neg E$

| No. | $S$ | $E$ | $H$ | $S \lor E$ | $S \longrightarrow H$ | $E \longrightarrow \neg H$ | $\neg (S \land E)$ |
| --: | :-: | :-: | :-: | :--------: | :-------------------: | :------------------------: | :----------------: |
|   1 |  F  |  F  |  F  |     F      |           T           |             T              |         T          |
|   2 |  F  |  F  |  T  |     F      |           T           |             T              |         T          |
|   3 |  F  |  T  |  F  |     T      |           T           |             T              |         T          |
|   4 |  T  |  T  |  T  |     T      |           T           |             F              |         F          |
|   5 |  T  |  F  |  F  |     T      |           F           |             T              |         T          |
|   6 |  T  |  F  |  T  |     T      |           T           |             T              |         T          |
|   7 |  T  |  T  |  F  |     T      |           F           |             T              |         F          |
|   8 |  T  |  T  |  T  |     T      |           T           |             F              |         F          |

- (b) If the tax rate and the unemployment rate both go up, then there will be a recession. If the GNP goes up, then there will not be a recession. The GNP and taxes are both going up. Therefore, the unemployment rate is not going up.

  Let $T$ be "the tax rate goes up", $U$ be "the unemployment rate goes up", $R$ be "there will be a recession", $G$ be "GNP goes up"

  $(T \land U) \longrightarrow R$

  $G \longrightarrow \neg R$

  $G \land T$

  $-------$

  $\therefore \neg U$

| No. | $T$ | $U$ | $G$ | $R$ | $(T \land U) \longrightarrow R$ | $G \longrightarrow \neg R$ | $G \land T$ | $\neg U$ |
| --: | :-: | :-: | :-: | :-: | :-----------------------------: | :------------------------: | :---------: | :------: |
|   1 |  F  |  F  |  F  |  F  |                T                |             T              |      F      |    T     |
|   2 |  F  |  F  |  F  |  T  |                T                |             T              |      F      |    T     |
|   3 |  F  |  F  |  T  |  F  |                T                |             T              |      F      |    T     |
|   4 |  F  |  F  |  T  |  T  |                T                |             F              |      F      |    T     |
|   5 |  F  |  T  |  F  |  F  |                T                |             T              |      F      |    F     |
|   6 |  F  |  T  |  F  |  T  |                T                |             T              |      F      |    F     |
|   7 |  F  |  T  |  T  |  F  |                T                |             T              |      F      |    F     |
|   8 |  F  |  T  |  T  |  T  |                T                |             F              |      F      |    F     |
|   9 |  T  |  F  |  F  |  F  |                T                |             T              |      F      |    T     |
|  10 |  T  |  F  |  F  |  T  |                T                |             T              |      F      |    T     |
|  11 |  T  |  F  |  T  |  F  |                T                |             T              |      T      |    T     |
|  12 |  T  |  F  |  T  |  T  |                T                |             F              |      T      |    T     |
|  13 |  T  |  T  |  F  |  F  |                F                |             T              |      F      |    F     |
|  14 |  T  |  T  |  F  |  T  |                T                |             T              |      F      |    F     |
|  15 |  T  |  T  |  T  |  F  |                F                |             T              |      T      |    F     |
|  16 |  T  |  T  |  T  |  T  |                T                |             F              |      T      |    F     |

- (c) Thewarning light will come on if and only if the pressure is too high and the relief valve is clogged. The relief valve is not clogged. Therefore, the warning light will come on if and only if the pressure is too high.

#### 5.

- (a) Show that $P \iff Q$ is equivalent to $(P \land Q) \lor (\neg P \land\neg Q)$.

  $P \iff Q$

  $(P \implies Q) \land (Q \implies P)$ (Definition of $\iff$)

  $(\neg P \lor Q) \land (\neg P \implies \neg Q)$ (Definition of $\implies$, contrapositive law)

  $(\neg P \lor Q) \land \neg(\neg P \land \neg(\neg Q))$

  $(\neg P \lor Q) \land (P \lor \neg Q)$

- (b) Show that $(P \implies Q) \lor (P \implies R)$ is equivalent to $P \implies (Q \lor R)$.
